src/bvm_extras.lean
@@ -179,6 +179,12 @@ end
 /-- The successor operation on sets (in particular von Neumman ordinals) -/
 @[reducible]def succ (x : bSet 𝔹) := bSet.insert1 x x
 
+@[simp]lemma subset_succ {x : bSet 𝔹} {Γ} : Γ ≤ x ⊆ᴮ (succ x) :=
+begin
+  rw subset_unfold', bv_intro z, bv_imp_intro Hz, erw mem_insert1,
+  from bv_or_right ‹_›
+end
+
 lemma succ_eq_binary_union {x : bSet 𝔹} {Γ} : Γ ≤ succ x =ᴮ binary_union {x} x :=
 begin
   simp[succ, binary_union], apply mem_ext,
